testdata/out/goose/github_com/mjschwenne/grackle/testdata/out/go/completeslice_gk.v
@@ -13,7 +13,7 @@ Definition S := struct.decl [
 ].
 
 Definition Marshal: val :=
-  rec: "Marshal" "c" "prefix" :=
+  rec: "Marshal" "prefix" "c" :=
     let: "enc" := ref_to (slice.T byteT) "prefix" in
     let: "strgBytes" := StringToBytes (struct.get S "Strg" "c") in
     "enc" <-[slice.T byteT] (marshal.WriteInt (![slice.T byteT] "enc") (slice.len "strgBytes"));;
